- Added some additional value locales in utp_value mirroring those in utp_sorts. - Extend expressions with various constructs, including substitutions and predicate marshalling. - Added designs in a preliminary form.

theories/generic/utp_expression.thy
@@ -7,16 +7,19 @@
 header {* Generic Expressions *}
 
 theory utp_expression
-imports "../utp_types" utp_gen_pred utp_eval_tactic utp_value
+imports "../utp_types" "../utp_sorts" utp_gen_pred utp_eval_tactic utp_value
 begin
 
+type_synonym ('VALUE, 'TYPE) BINDING_VAL =
+  "('VALUE, 'TYPE) BINDING \<Rightarrow> 'VALUE option"
+
 type_synonym ('VALUE, 'TYPE) EXPRESSION =
-  "(('VALUE, 'TYPE) BINDING \<Rightarrow> 'VALUE option) \<times> 'TYPE"
+  "('VALUE, 'TYPE) BINDING_VAL \<times> 'TYPE"
 
 type_synonym ('VALUE, 'TYPE) ALPHA_EXPRESSION =
   "('TYPE ALPHABET) \<times> ('VALUE, 'TYPE) EXPRESSION"
 
-abbreviation expr_body :: "('VALUE, 'TYPE) ALPHA_EXPRESSION \<Rightarrow> (('VALUE, 'TYPE) BINDING \<Rightarrow> 'VALUE option)" where
+abbreviation expr_body :: "('VALUE, 'TYPE) ALPHA_EXPRESSION \<Rightarrow> ('VALUE, 'TYPE) BINDING_VAL" where
 "expr_body x \<equiv> fst (snd x)"
 
 abbreviation expr_type :: "('VALUE, 'TYPE) ALPHA_EXPRESSION \<Rightarrow> 'TYPE" where
@@ -27,7 +30,8 @@ abbreviation expr_alpha :: "('VALUE, 'TYPE) ALPHA_EXPRESSION \<Rightarrow> ('TYP
 
 notation expr_alpha ("\<alpha>e")
 
-context GEN_PRED
+locale GEN_EXPR = GEN_PRED "type_rel" + BOOL_VALUE "type_rel"
+  for type_rel :: "'VALUE :: BOOL_SORT \<Rightarrow> 'TYPE \<Rightarrow> bool" (infix ":" 50)
 begin
 
 subsection {* Expressions *}
@@ -40,21 +44,53 @@ definition WF_ALPHA_EXPR :: "('VALUE, 'TYPE) ALPHA_EXPRESSION set" where
                    \<and> (\<forall> b1 \<in> WF_BINDING. \<forall> b2 \<in> WF_BINDING. 
                       b1 \<cong> b2 on \<alpha>e e \<longrightarrow> expr_body e b1 = expr_body e b2)}"
 
+definition wfexpr_body :: "('VALUE, 'TYPE) ALPHA_EXPRESSION \<Rightarrow> (('VALUE, 'TYPE) BINDING \<Rightarrow> 'VALUE)" ("\<beta>e") where
+"x \<in> WF_ALPHA_EXPR \<longrightarrow> wfexpr_body x v = the (expr_body x v)"
+
 subsection {* Operators *}
 
 definition VarE :: "'TYPE VAR \<Rightarrow> ('VALUE, 'TYPE) ALPHA_EXPRESSION" where
 "VarE v \<equiv> ({v}, (\<lambda> b. Some (b v), var_type v))"
 
+(* Should this definition using the definite description operator or should we be
+   able to infer a type? *)
+definition LitE :: "'VALUE \<Rightarrow> ('VALUE, 'TYPE) ALPHA_EXPRESSION" where
+"LitE v \<equiv> ({}, (\<lambda> b. Some v, SOME t. v : t))"
+
+definition TrueE :: "('VALUE, 'TYPE) ALPHA_EXPRESSION" ("true") where
+"TrueE \<equiv> LitE (MkBool True)"
+
+definition FalseE :: "('VALUE, 'TYPE) ALPHA_EXPRESSION" ("false") where
+"FalseE \<equiv> LitE (MkBool False)"
+
+(* These functions for the time being are assumed to be closed, but this should change *)
+definition UopE :: "('VALUE \<Rightarrow> 'VALUE) \<Rightarrow>
+                    ('VALUE, 'TYPE) ALPHA_EXPRESSION \<Rightarrow> 
+                    ('VALUE, 'TYPE) ALPHA_EXPRESSION" where
+"UopE f x = (\<alpha>e x, (\<lambda> b. Option.map f (expr_body x b), expr_type x))"
+
+definition BopE :: "('VALUE \<Rightarrow> 'VALUE \<Rightarrow> 'VALUE) \<Rightarrow>
+                    ('VALUE, 'TYPE) ALPHA_EXPRESSION \<Rightarrow> 
+                    ('VALUE, 'TYPE) ALPHA_EXPRESSION \<Rightarrow>
+                    ('VALUE, 'TYPE) ALPHA_EXPRESSION" where
+"BopE f x y = (\<alpha>e x \<union> \<alpha>e y, (\<lambda> b. case (expr_body x b,expr_body y b) 
+                                    of (Some a,Some b) \<Rightarrow> Some (f a b)
+                                       | _ \<Rightarrow> None), expr_type x)"
+
+definition PredE :: "('VALUE, 'TYPE) ALPHA_PREDICATE \<Rightarrow> ('VALUE, 'TYPE) ALPHA_EXPRESSION" where
+"p \<in> WF_ALPHA_PREDICATE \<longrightarrow> PredE p = (\<alpha> p, (\<lambda> b. Some (MkBool (b \<in> \<beta> p))), BoolType)"
+
 subsection {* Predicates *}
 
-(*
 definition ExprP :: "('VALUE, 'TYPE) ALPHA_EXPRESSION \<Rightarrow> ('VALUE, 'TYPE) ALPHA_PREDICATE" where
-"expr_type e = BoolType \<longrightarrow> ExprP e \<equiv> e" 
-*)
+"(expr_type e = BoolType) \<longrightarrow> ExprP e = (\<alpha>e e , {b. b \<in> WF_BINDING \<and> (\<exists> t. (expr_body e) b = Some t \<and> DestBool t = True)})"
+
+abbreviation VarP ::  "'TYPE VAR \<Rightarrow> ('VALUE, 'TYPE) ALPHA_PREDICATE" ("&") where
+"VarP v \<equiv> ExprP (VarE v)"
 
 definition EqualP :: "('VALUE, 'TYPE) ALPHA_EXPRESSION \<Rightarrow> ('VALUE, 'TYPE) ALPHA_EXPRESSION \<Rightarrow> ('VALUE, 'TYPE) ALPHA_PREDICATE" where
 "e \<in> WF_ALPHA_EXPR \<and> f \<in> WF_ALPHA_EXPR \<longrightarrow> 
- EqualP e f = (\<alpha>e e \<union> \<alpha>e f, {b. b \<in> WF_BINDING \<and> (expr_body e b = expr_body f b)})"
+ EqualP e f = (\<alpha>e e \<union> \<alpha>e f, {b. b \<in> WF_BINDING \<and> (\<beta>e e b = \<beta>e f b)})"
 
 notation EqualP (infixr "==p" 150)
 
@@ -63,29 +99,83 @@ abbreviation EqualVP :: "'TYPE VAR \<Rightarrow> ('VALUE, 'TYPE) ALPHA_EXPRESSIO
 
 notation EqualVP (infixr "=p" 150)
 
-subsubsection {* Alphabet Theorems *}
-
-lemma VarP_alphabet [simp]: "\<alpha>e (VarE v) = {v}"
-  by (simp add:VarE_def)
-
-lemma EqualP_alphabet [simp]: 
-"\<lbrakk> e \<in> WF_ALPHA_EXPR; f \<in> WF_ALPHA_EXPR \<rbrakk> \<Longrightarrow> \<alpha> (e ==p f) = \<alpha>e e \<union> \<alpha>e f"
-  by (simp add:EqualP_def)
+(* Coarse substitution *)
+definition SubsP :: "('VALUE, 'TYPE) ALPHA_PREDICATE \<Rightarrow> ('VALUE, 'TYPE) ALPHA_EXPRESSION \<Rightarrow> 'TYPE VAR \<Rightarrow> ('VALUE, 'TYPE) ALPHA_PREDICATE" ("_[_|_]" [200]) where
+"x \<notin> \<alpha>e e \<longrightarrow> SubsP p e x = (\<exists>-p {x} . p \<and>p (x =p e))"
 
 subsubsection {* Closure Theorems *}
 
-lemma VarE_closure[simp]:
+lemma ExprP_closure[closure]:
+"\<lbrakk> e \<in> WF_ALPHA_EXPR; expr_type e = BoolType \<rbrakk> \<Longrightarrow> 
+ ExprP e \<in> WF_ALPHA_PREDICATE"
+  by (auto simp add:ExprP_def WF_ALPHA_EXPR_def WF_ALPHA_PREDICATE_def WF_BINDING_SET_def)
+
+lemma VarE_closure[closure]:
 "VarE v \<in> WF_ALPHA_EXPR"
   by (simp add:VarE_def WF_ALPHA_EXPR_def WF_BINDING_def beta_equiv_def alpha_closure var)
 
-lemma EqualP_closure[simp]: 
+lemma LitE_closure[closure]:
+"LitE v \<in> WF_ALPHA_EXPR"
+proof -
+  obtain t where "v : t" by (metis type_rel_total)
+  hence "op : v (Eps (op : v))"
+    by (auto intro:someI)
+
+  thus ?thesis
+    by (simp add:LitE_def alpha_closure WF_ALPHA_EXPR_def)
+qed
+
+lemma EqualP_closure[closure]: 
 "\<lbrakk> e \<in> WF_ALPHA_EXPR; f \<in> WF_ALPHA_EXPR \<rbrakk> \<Longrightarrow>
  e ==p f \<in> WF_ALPHA_PREDICATE"
-  apply (simp add:EqualP_def WF_ALPHA_EXPR_def WF_ALPHA_PREDICATE_def WF_BINDING_SET_def)
+  apply (simp add:EqualP_def WF_ALPHA_EXPR_def WF_ALPHA_PREDICATE_def WF_BINDING_SET_def wfexpr_body_def)
   apply (simp add:alpha_closure var beta_equiv_union)
   apply (auto)
 done
+
+lemma EqualVP_closure[closure]: 
+"\<lbrakk> e \<in> WF_ALPHA_EXPR; x \<notin> \<alpha>e e \<rbrakk> \<Longrightarrow>
+ x =p e \<in> WF_ALPHA_PREDICATE"
+  by (simp add:closure)
+
+lemma SubsP_closure[closure]:
+"\<lbrakk> p \<in> WF_ALPHA_PREDICATE; e \<in> WF_ALPHA_EXPR; x \<notin> \<alpha>e e \<rbrakk> \<Longrightarrow>
+ p[e|x] \<in> WF_ALPHA_PREDICATE"
+  by (simp add:SubsP_def closure alpha_closure)
+
+subsubsection {* Alphabet Theorems *}
+
+lemma VarP_alphabet [alphabet]: "\<alpha>e (VarE v) = {v}"
+  by (simp add:VarE_def)
+
+lemma EqualP_alphabet [alphabet]: 
+"\<lbrakk> e \<in> WF_ALPHA_EXPR; f \<in> WF_ALPHA_EXPR \<rbrakk> \<Longrightarrow> \<alpha> (e ==p f) = \<alpha>e e \<union> \<alpha>e f"
+  by (simp add:EqualP_def)
+
+lemma LitE_alphabet [alphabet]:
+"\<alpha>e (LitE v) = {}" by (simp add:LitE_def)
+
+lemma ExprP_alphabet [alphabet]:
+"\<lbrakk> e \<in> WF_ALPHA_EXPR; expr_type e = BoolType \<rbrakk> \<Longrightarrow> \<alpha> (ExprP e) = \<alpha>e e"
+  by (simp add:ExprP_def)
+
+lemma SubsP_alphabet [alphabet]:
+"\<lbrakk> p \<in> WF_ALPHA_PREDICATE; e \<in> WF_ALPHA_EXPR; x \<notin> \<alpha>e e \<rbrakk> \<Longrightarrow> 
+ \<alpha> (p[e|x]) = (\<alpha> p \<union> \<alpha>e e) - {x}"
+  by (simp add:SubsP_def alphabet closure alpha_closure)
+
+subsubsection {* Binding Theorems *}
+
+lemma VarE_binding[simp]: "b \<in> WF_BINDING \<Longrightarrow> \<beta>e (VarE x) b = b x"
+  apply(simp add:wfexpr_body_def closure)
+  apply(simp add:VarE_def)
+done
   
+subsubsection {* Typing Theorems *}
+
+lemma VarE_type: "expr_type (VarE v) = type v"
+  by (simp add:VarE_def)
+
 subsubsection {* Equality Theorems *}
 
 lemma EqualP_refl: "e \<in> WF_ALPHA_EXPR \<Longrightarrow> taut (e ==p e)"
@@ -112,8 +202,57 @@ lemma EqualP_trans:
   apply(force)
 done
 
+(*
 declare EqualP_def [eval]
 declare VarE_def [eval]
+*)
+
+lemma EvalP_EqualVP[eval]: "\<lbrakk> e \<in> WF_ALPHA_EXPR; b \<in> WF_BINDING \<rbrakk> \<Longrightarrow> EvalP (x =p e) b \<longleftrightarrow> (b x = \<beta>e e b)"
+  apply(simp add:EvalP_def closure)
+  apply(simp add:EqualP_def alpha_closure closure)
+done
+
+lemma expr_body_weaken[simp]: "\<lbrakk> e \<in> WF_ALPHA_EXPR; v \<notin> \<alpha>e e; b \<in> WF_BINDING; b' \<in> WF_BINDING \<rbrakk> \<Longrightarrow> \<beta>e e (b \<oplus> b' on {v}) = \<beta>e e b"
+  apply(simp add:wfexpr_body_def)
+  apply(auto simp add: WF_ALPHA_EXPR_def)
+  apply(subgoal_tac "b \<oplus> b' on {v} \<cong> b on \<alpha>e e")
+  apply(erule_tac ballE)
+  apply(erule_tac x="b \<oplus> b' on {v}" in ballE)
+  apply(erule_tac x="b" in ballE)
+  apply(auto)
+  apply (metis Int_empty_left Int_insert_left beta_equiv_override_2)
+done
+
+(* Quick sanity check *)
+lemma SubsP_AndP: "\<lbrakk> p \<in> WF_ALPHA_PREDICATE; q \<in> WF_ALPHA_PREDICATE; e \<in> WF_ALPHA_EXPR; x \<notin> \<alpha>e e \<rbrakk> \<Longrightarrow>
+       (p \<and>p q)[e|x] = p[e|x] \<and>p q[e|x]"
+  apply(simp add:SubsP_def)
+  apply(intro eval_intro)
+  apply(blast intro:closure alpha_closure)
+  apply(blast intro:closure alpha_closure)
+  apply(force simp add:alphabet closure alpha_closure)
+  apply(simp add:eval closure alpha_closure)
+  apply(auto)
+  apply(rule_tac x="b'" in bexI)
+  apply(auto)
+  apply(subgoal_tac "b' \<cong> b'a on {x}")
+  apply (metis (hide_lams, no_types) beta_equiv_override beta_equiv_override_3 override_on_cancel3')
+  apply(auto)
+done
+
+lemma SubsP_VarP: 
+"\<lbrakk> e \<in> WF_ALPHA_EXPR; x \<notin> \<alpha>e e; expr_type e = BoolType; type x = BoolType \<rbrakk> 
+\<Longrightarrow> (VarP x)[e|x] = ExprP e"
+  apply(rule eval_intro)
+  apply(simp add:closure alpha_closure VarE_type)
+  apply(simp add:closure alpha_closure VarE_type)
+  apply(simp add:alphabet closure alpha_closure VarE_type)
+  apply(simp add:eval closure alpha_closure VarE_type SubsP_def)
+  apply(rule ballI)
+  apply(rule iffI)
+  apply(simp add:VarE_def VarE_type)
+sorry
+
 
 end
 end
